Some stuff when group 2 was giving me trouble

project2/strings2.dfy
@@ -31,73 +31,88 @@ lemma PrefixNegationLemma(pre:string, str:string)
 
 
 
-
-
-
-
-
-
-
 // Excplicit char by char checking in the substrings
+/*
 predicate isSubstringPred(sub:string, str:string)
 {
-	|str| >= |sub| && exists k :: (0 <= k <= (|str| - |sub|) 
-		==> (forall x :: k <= x < k+|sub| ==> str[x] == sub[x-k]))
+	|str| >= |sub| && 
+	exists k :: (0 <= k <= (|str| - |sub|) ==> 
+		(forall x :: k <= x < k+|sub| ==> str[x] == sub[x-k]))
 
 }
+*/
+
 
 // Using prefix predicate
-predicate isSubstringPred2(sub:string, str:string) {
-	|str| >= |sub| && exists k :: (0 <= k <= (|str| - |sub|) 
+predicate isSubstringPredUsingPrefix(sub:string, str:string) {
+	|str| >= |sub| && |sub| != 0 && 
+	exists k :: (0 <= k <= (|str| - |sub|) 
 		==> isPrefixPred(sub, str[k..]))
 }
 
+
 // Using sublists
-predicate isSubstringPred3(sub:string, str:string) {
-	|str| >= |sub| && exists k :: (0 <= k <= (|str| - |sub|) 
+predicate isSubstringPred(sub:string, str:string) {
+	|str| >= |sub| && |sub| != 0 && |str| != 0 && 
+	exists k :: (0 <= k <= (|str| - |sub|) 
 		==> str[k..][..|sub|] == sub)
 }
 
+predicate isSubstringPredRowan(sub:string, str:string) {
+	(|sub| <= |str|) && (|sub| != 0) && (|str| != 0) && 
+	exists x :: (0 <= x <= (|str|-|sub|) 
+		==> exists y :: (y == (|sub| + x) ==> str[x..y]==sub))
+}
+
+
 lemma substringPredsAggreee(sub:string, str:string) 
-	//ensures isSubstringPred(sub, str) <==> isSubstringPred2(sub, str) 
-	//ensures isSubstringPred2(sub, str) <==> isSubstringPred3(sub, str) 
-	//ensures isSubstringPred(sub, str) ==> isSubstringPred3(sub, str)
-	//ensures isSubstringPred3(sub, str) ==> isSubstringPred(sub, str) 
+	//ensures isSubstringPred(sub, str) <==> isSubstringPredRowan(sub, str) 
+	//ensures isSubstringPred(sub, str) ==> isSubstringPredUsingPrefix(sub, str) 
+	//ensures isSubstringPredRowan(sub, str) <==> isSubstringPredUsingPrefix(sub, str)
+	//ensures isSubstringPredUsingPrefix(sub, str) ==> isSubstringPred(sub, str) 
 {}
 
 
-predicate isNotSubstringPred(sub:string, str:string)
-{
-	|sub| > |str| && !isSubstringPred(sub, str)
+
+// Using sublists
+predicate isNotSubstringPred(sub:string, str:string) {
+	|str| < |sub| || |sub| == 0 || |str| == 0 || 
+	forall k :: (0 <= k <= (|str| - |sub|) 
+		==> str[k..][..|sub|] != sub)
 }
 
+/*
 predicate isNotSubstringPred3(sub:string, str:string)
 {
 	|str| < |sub| || !(exists k :: (0 <= k <= (|str| - |sub|) 
 		==> str[k..][..|sub|] == sub))
 }
+*/
 
+
+/*
+predicate test(str:string, sub:string) {
+	|str| >= |sub| &&
+	forall x :: 0 <= x <= (|str| - |sub|) ==>
+		forall y :: 0 <= y <= |sub| ==>
+			forall z :: z == x + y ==> 
+				str[x..z] == str[x..][..y]
+}
+*/
 
 lemma SubstringNegationLemmaExpanded(sub:string, str:string) 
 	ensures isSubstringPred(sub,str) ==> !isNotSubstringPred(sub,str)		// is substring, but not not a substring
-	ensures !isNotSubstringPred(sub,str) ==> isSubstringPred(sub,str)
-	ensures !isSubstringPred(sub,str) ==>  isNotSubstringPred(sub,str)
-	ensures isNotSubstringPred(sub,str) ==> !isSubstringPred(sub,str)
+	//ensures !isNotSubstringPred(sub,str) ==> isSubstringPred(sub,str)
+	//ensures !isSubstringPred(sub,str) ==>  isNotSubstringPred(sub,str)
+	//ensures isNotSubstringPred(sub,str) ==> !isSubstringPred(sub,str)
 {}
 
 // Sanity check: Dafny should be able to automatically prove the following lemma
+
 lemma SubstringNegationLemma(sub:string, str:string)
 	ensures  isSubstringPred(sub,str) <==> !isNotSubstringPred(sub,str)
 	ensures !isSubstringPred(sub,str) <==>  isNotSubstringPred(sub,str)
 {}
-
-lemma SubstringNegationLemmaExpanded3(sub:string, str:string) 
-	ensures isSubstringPred3(sub,str) ==> !isNotSubstringPred3(sub,str)		// is substring, but not not a substring
-	ensures !isNotSubstringPred3(sub,str) ==> isSubstringPred3(sub,str)
-	ensures !isSubstringPred3(sub,str) ==>  isNotSubstringPred3(sub,str)
-	ensures isNotSubstringPred3(sub,str) ==> !isSubstringPred3(sub,str)
-{}
-
 
 
 
