project2/test.dfy
@@ -1,0 +1,31 @@
+// Test whether the chain of subsequences works
+method Main() {
+  var str := "dogcat";
+	var sub := "at";
+  
+  var stop := |str| - |sub|;  // 4 --> stop at 'a'
+  var i := 0;
+  
+  while (i <= stop) {
+    print str[i..][..|sub|];
+    print "\n";
+    i := i+1;
+  }
+  
+
+  assert str[5..][..1] == str[5..6];
+  //assert  (indexed == split);
+}
+
+predicate test(x:nat) {
+  x == 5
+}
+
+predicate test2(x:nat) {
+  x > 4 && x < 6
+}
+
+lemma lem(x:nat) 
+  ensures test(x) <==> test2(x) 
+  ensures !test(x) <==> !test2(x)
+{}
