project2/vas.dfy
@@ -1,0 +1,63 @@
+predicate isPrefixPred(pre:string, str:string)
+{
+	(|pre| <= |str|) && pre == str[..|pre|]
+}
+
+
+// Build each substring of length |sub| by walking through the sequence
+predicate isSubstringPred(sub:string, str:string)
+{
+  |sub| <= |str| && |sub| > 0 && 
+		exists x :: (0 <= x <= (|str|-|sub|) ==> exists y :: (y == (|sub| + x) ==> str[x..y]==sub)) 
+}
+
+// Same thing just without needing to explicitly define y
+predicate isSubstringPredChainSubs(sub:string, str:string) {
+	|sub| <= |str| && |sub| > 0 && 
+		exists x :: 0 <= x <= (|str|-|sub|) && (str[x..][..|sub|]) == sub
+}
+
+// Same thing using prefix method
+predicate isSubstringPredPrefix(sub:string, str:string) {
+		exists x :: 0 <= x <= (|str|-|sub|) && isPrefixPred(sub, str[x..])
+}
+
+lemma test2(str:string, x:nat, y:nat)
+requires x >= 0 && x < |str| &&  (x+y) >= 0 && (x+y) < |str|
+ensures str[x..y+x] == str[x..][..y]
+{}
+
+// Rustan Leino -- Verification Corner - Writing inductive proofs
+// Rustan leino imperial and Sofia Drossopoulou
+
+lemma test(sub:string, str:string)
+
+  // Right and chain subs
+  //ensures isSubstringPredChainSubs(sub, str) ==> isSubstringPred(sub, str) 
+  //ensures isSubstringPred(sub, str) <==> isSubstringPredChainSubs(sub, str) 
+
+  // Right and prefix call
+  //ensures isSubstringPred(sub, str) ==> isSubstringPredPrefix(sub, str)
+  ensures isSubstringPredPrefix(sub, str) ==> isSubstringPred(sub, str) 
+  //ensures isSubstringPred(sub, str) <==> isSubstringPredPrefix(sub, str) 
+
+  // Chain Subs and Prefix call
+  //ensures isSubstringPredChainSubs(sub, str) ==> isSubstringPredPrefix(sub, str)
+  //ensures isSubstringPredPrefix(sub, str) ==> isSubstringPredChainSubs(sub, str) 
+  //ensures isSubstringPredChainSubs(sub, str) <==> isSubstringPredPrefix(sub, str) 
+{
+}
+
+predicate isNotSubstringPred(sub:string, str:string)
+{
+	|sub| > |str| || |sub| == 0 || |str| == 0  || 
+		forall x :: !(0 <= x <= (|str|-|sub|) ==> 
+    exists y :: (y == (|sub| + x) ==> str[x..y]==sub))
+}
+
+// Sanity check: Dafny should be able to automatically prove the following lemma
+lemma SubstringNegationLemma(sub:string, str:string)
+	ensures  isSubstringPred(sub,str) <==> !isNotSubstringPred(sub,str)
+	ensures  isSubstringPredPrefix(sub,str) <== !isNotSubstringPred(sub,str)
+	//ensures !isSubstringPredPrefix(sub,str) <==>  isSubstringPredPrefix(sub,str)
+{}
